Verbatim/actions/impl.v
@@ -1,0 +1,130 @@
+From Verbatim Require Import state.
+Require Import List.
+Import ListNotations.
+
+From Verbatim Require Import ltac.
+
+
+
+Module Type LEXER (STT : state.T).
+
+  Export STT.Defs.
+  Export STT.R.Defs.
+  Export STT.Ty.
+
+  Parameter lex : list Rule -> String -> list Token * String.
+  
+  Parameter lex_sound :  forall ts code rest rus,
+      lex rus code = (ts, rest)
+      -> rules_is_function rus
+      -> tokenized rus code ts rest.
+  
+  Parameter lex_complete : forall ts code rest rus,
+      tokenized rus code ts rest
+      -> rules_is_function rus
+      -> lex rus code = (ts, rest).
+
+End LEXER.
+
+Module Type SEM_USER (Import STT : state.T).
+
+  Import STT.R.Defs.
+  Import STT.R.
+  Import STT.Defs.
+  Import STT.Ty.
+  
+  Parameter sem_ty : Label -> Type.
+  Parameter apply_sem : (Label * String) -> option {l : Label & sem_ty l}.
+  Parameter label_carries : forall l l' s t,
+      apply_sem (l, s) = Some (existT _ l' t)
+      -> l = l'.
+
+End SEM_USER.
+
+Module SemLexerFn (STT : state.T) (Export LXR : LEXER STT) (Import USER : SEM_USER STT).
+
+  
+  Module Import Core.
+    
+    Definition sem_token := {l : Label & sem_ty l}.
+
+  End Core. 
+
+  Module Import Spec.
+      
+    Inductive tokenized_sem' (rus : list Rule) : String -> (list (option sem_token))
+                                                -> String -> Prop :=
+    | Tkd_sem'_Nil (code : String)
+               (H : tokenized rus code [] code)
+      : tokenized_sem' rus code [] code
+    | Tkd_sem'_Cons (t : option sem_token) (ts : list (option sem_token))
+               (l : Label) (p : Prefix) (s0 s1 : Suffix)
+               (Hsem : apply_sem (l, p) = t)
+               (* the first token matches the input *)
+               (H0 : first_token (p ++ s0 ++ s1) rus (l,p))
+               (* The rest of the tokens match the rest of the input *)
+               (IH : tokenized_sem' rus (s0 ++ s1) ts s1) :
+        tokenized_sem' rus (p ++ s0 ++ s1) (t :: ts) s1.
+
+    Inductive tokenized_sem (rus : list Rule) : String -> (option (list sem_token))
+                                                -> String -> Prop :=
+      (* The Some case really needs some work, probably another predicate *)
+    | Tkd_sem_Some (code rest : String) (ts : list Token) (sts : list sem_token)
+                   (n : nat) (st st' : sem_token) (t : Token)
+                   (H0 : tokenized rus code ts rest)
+                   (H3 : (nth_error ts n = Some t
+                         /\ nth_error sts n = Some st)
+                         -> (apply_sem t = Some st' /\ st = st'))
+                   (H6 : length ts = length sts)
+      : tokenized_sem rus code (Some sts) rest
+    | Tkd_sem_None (code rest : String) (t : Token) (ts : list Token)
+        (H : tokenized rus code ts rest)
+        (Hin : In t ts)
+        (Hsem : apply_sem t = None)
+      : tokenized_sem rus code None rest.
+    
+  End Spec.
+
+  Module Import Impl.
+
+    Definition lex_sem' (rus : list Rule) (code : String) : (list (option sem_token)) * String :=
+      match lex rus code with
+      | (ts, rest) => ((map apply_sem ts), rest)
+      end.
+
+    Fixpoint lo2ol {A : Type} (xs : list (option A)) : option (list A) :=
+      match xs with
+      | [] => Some []
+      | None :: ys => None
+      | Some x :: ys =>
+        match lo2ol ys with
+        | None => None
+        | Some zs => Some (x :: zs)
+        end
+      end.
+
+    Definition lex_sem (rus : list Rule) (code : String) : (option (list sem_token)) * String :=
+      match lex_sem' rus code with
+      | (ts, rest) => (lo2ol ts, rest)
+      end.
+
+  End Impl.
+
+  Module Correct.
+
+    Theorem lex_sem_sound : forall o code rest rus,
+      lex_sem rus code = (o, rest)
+      -> rules_is_function rus
+      -> tokenized_sem rus code o rest.
+    Proof.
+      intros. destruct o.
+      {
+        unfold lex_sem in *. unfold lex_sem' in *. repeat dm. repeat inj_all.
+        eapply Tkd_sem_Some; eauto.
+        - eapply lex_sound; eauto.
+        - Abort.
+
+  End Correct.
+
+End SemLexerFn.
+  
