Verbatim/actions/instance.v
@@ -1,0 +1,211 @@
+Require Import List.
+Import ListNotations.
+
+Require Import String.
+Open Scope string_scope.
+Require Import Ascii.
+
+Require Import BinInt.
+Require Import PrimFloat.
+
+Require Import DecimalString.
+Import NilEmpty.
+
+From Verbatim Require ExampleLexer.
+Import ExampleLexer.MEM.STT.R.Defs.
+From Verbatim Require FloatLexer.
+Import FloatLexer.Splitter.
+From Verbatim Require Import actions.impl.
+
+From Verbatim Require Import ltac.
+
+
+Module Import STT <: state.T := ExampleLexer.MEM.STT.
+
+Module Import LXR <: LEXER STT.
+
+  Definition lex := ExampleLexer.C.IMPL.Lex.lex_M.
+  Definition lex_sound := ExampleLexer.C.lex_sound__M.
+  Definition lex_complete := ExampleLexer.C.lex_complete__M.
+
+End LXR.
+
+Module USER <: SEM_USER STT.
+
+  Definition sem_ty (l : Label) : Type :=
+    match l with
+    | INT => Z
+    | FLOAT => float
+    | STRING => string
+    | TRUE => unit
+    | FALSE => unit
+    | NULL => unit
+    | COLON => unit
+    | COMMA => unit
+    | LEFT_BRACKET => unit
+    | RIGHT_BRACKET => unit
+    | LEFT_BRACE => unit
+    | RIGHT_BRACE => unit
+    | WS => unit
+    end.
+
+
+  Set Printing All.
+  Compute "0".
+  Compute "-".
+  Unset Printing All.
+
+  (* Doesn't check for leading 0 or -0 *)
+  Definition String2uint' (z : String) : option Z :=
+    match z with
+    | [] => None
+    | _ =>        
+      match uint_of_string (string_of_list_ascii z) with
+      | None => None
+      | Some x => Some (Z.of_uint x)
+      end
+    end.
+
+  (* Doesn't check for leading 0 or -0 *)
+  Definition String2int' (z : String) : option Z :=
+    match z with
+    | [] => None
+    | _ =>        
+      match int_of_string (string_of_list_ascii z) with
+      | None => None
+      | Some x => Some (Z.of_int x)
+      end
+    end.
+
+  Definition String2int (z : String) : option Z :=
+    match z with
+    (* Just a 0 *)
+    | [Ascii false false false false true true false false] => Some 0%Z
+    (* Just a -0 *)
+    | [Ascii true false true true false true false false ;
+      Ascii false false false false true true false false] => Some 0%Z
+    (* Leading 0 *)
+    | Ascii false false false false true true false false :: _ => None
+    (* Only a - *)
+    | [Ascii true false true true false true false false] => None
+    (* Leading -0 *)
+    | Ascii true false true true false true false false ::
+            Ascii false false false false true true false false :: _ => None
+    | _ => String2int' z
+    end.
+
+
+
+  Fixpoint float_exp_pos (f : float) (n : nat) : float :=
+    match n with
+    | 0 => 1%float
+    | S m => f * (float_exp_pos f m)
+    end.
+
+  Definition float_exp (f : float) (i : Z) : float :=
+    match i with
+    | Z0 => 1%float
+    | Zpos n => float_exp_pos f (Pos.to_nat n)
+    | Zneg n => 1%float / float_exp_pos f (Pos.to_nat n)
+    end.
+    
+  Definition String2float' (o : option (String * String * String)) : option float :=
+    match o with
+    | Some (i, [], []) =>
+      match String2int i with
+      | Some i' => Some (of_int63 (Int63.of_Z i'))
+      | None => None
+      end
+    | Some (i, d, []) =>
+      match String2int i with
+      | Some i' =>
+        match String2uint' d with
+        | Some d' =>
+          let
+            dec_factor := float_exp 10%float (Zneg (Pos.of_nat (List.length d)))
+          in
+          let
+            dec_part :=  ((of_int63 (Int63.of_Z d')) * dec_factor)%float
+          in
+          Some ((of_int63 (Int63.of_Z i')) + dec_part)%float
+        | None => None
+        end
+      | None => None
+      end
+    | Some (i, [], e) => 
+      match String2int i with
+      | Some i' =>
+        match String2int e with
+        | Some e' =>
+          let
+            exp_factor := float_exp 10%float e'
+          in
+          Some ((of_int63 (Int63.of_Z i')) * exp_factor)%float
+        | None => None
+        end
+      | None => None
+      end
+    | Some (i, d, e) => 
+      match String2int i with
+      | Some i' =>
+        match String2uint' d with
+        | Some d' =>
+          let
+            dec_factor := float_exp 10%float (Zneg (Pos.of_nat (List.length d)))
+          in
+          let
+            dec_part :=  ((of_int63 (Int63.of_Z d')) * dec_factor)%float
+          in
+          match String2int e with
+          | Some e' =>
+            let
+              exp_factor := float_exp 10%float e'
+            in
+            Some ((of_int63 (Int63.of_Z i') + dec_part) * exp_factor)%float
+          | None => None
+          end
+        | None => None
+        end
+      | None => None
+      end
+    | _ => None
+    end.
+
+  (* This is probably not super safe *)
+  Definition String2float (z : String) : option float :=
+    String2float' (Split_float_str z).
+
+  Definition toS (z : string) : String := list_ascii_of_string z.
+  Compute (String2float' (Some (toS "0", toS "3", toS "1"))).
+                   
+  
+  Definition apply_sem (pr : Label * String) : option {l : Label & sem_ty l} :=
+    match pr with
+    | (INT, z) =>
+      match (String2int z) with
+      | Some i => Some (existT sem_ty INT i)
+      | None => None
+      end
+    | (FLOAT, z) => 
+      match (String2float z) with
+      | Some i => Some (existT sem_ty FLOAT i)
+      | None => None
+      end
+    | (STRING, z) => Some (existT _ STRING "")  
+    | (L, _)      => Some (existT _ L tt)
+    end.
+
+  Compute (apply_sem (INT, toS "-3")).
+
+  Lemma label_carries : forall l l' s t,
+      apply_sem (l, s) = Some (existT sem_ty l' t)
+      -> l = l'.
+  Proof.
+    intros. destruct l; destruct l'; auto; sis; repeat dm; repeat inj_all; discriminate.
+  Qed.
+    
+End USER.
+
+Module Import SemLexer := SemLexerFn STT LXR USER.
+Import SemLexer.Impl.
+
